Add some defs/lemmas about events

src/program_proof/mvcc/mvcc_ghost.v
@@ -17,6 +17,7 @@ Local Definition key_vchainR := gmapR u64 vchainR.
 Local Definition tidsR := gmap_viewR u64 (leibnizO unit).
 Local Definition sid_tidsR := gmapR u64 tidsR.
 Local Definition sid_min_tidR := gmapR u64 mono_natR.
+Local Definition tid_modsR := gmap_viewR (u64 * (gmap u64 u64)) (leibnizO unit).
 
 Lemma sids_all_lookup (sid : u64) :
   int.Z sid < N_TXN_SITES ->
@@ -34,24 +35,40 @@ Class mvcc_ghostG Σ :=
     mvcc_key_vchainG :> inG Σ key_vchainR;
     mvcc_sid_tidsG :> inG Σ sid_tidsR;
     mvcc_sid_min_tidG :> inG Σ sid_min_tidR;
+    mvcc_abort_tids_ncaG :> inG Σ tidsR;
+    mvcc_abort_tids_faG :> inG Σ tidsR;
+    mvcc_abort_tids_fciG :> inG Σ tid_modsR;
+    mvcc_abort_tids_fccG :> inG Σ tid_modsR;
+    mvcc_commit_tidsG :> inG Σ tid_modsR;
   }.
 
 Definition mvcc_ghostΣ :=
   #[
      GFunctor key_vchainR;
      GFunctor sid_tidsR;
-     GFunctor sid_min_tidR
+     GFunctor sid_min_tidR;
+     GFunctor tidsR;
+     GFunctor tidsR;
+     GFunctor tid_modsR;
+     GFunctor tid_modsR;
+     GFunctor tid_modsR
    ].
 
 Global Instance subG_mvcc_ghostG {Σ} :
   subG mvcc_ghostΣ Σ → mvcc_ghostG Σ.
 Proof. solve_inG. Qed.
 
+(* TODO: remove the [mvcc_] prefix? *)
 Record mvcc_names :=
   {
     mvcc_key_vchain : gname;
     mvcc_sid_tids_gn : gname;
-    mvcc_sid_min_tid_gn : gname
+    mvcc_sid_min_tid_gn : gname;
+    mvcc_abort_tids_nca : gname;
+    mvcc_abort_tids_fa : gname;
+    mvcc_abort_tids_fci : gname;
+    mvcc_abort_tids_fcc : gname;
+    mvcc_commit_tids : gname
   }.
 
 Section definitions.
@@ -226,6 +243,257 @@ Proof.
 Qed.
 
 End definitions.
+
+
+Section event.
+
+Inductive event :=
+| EvCommit (tid : u64) (mods : gmap u64 u64)
+| EvRead   (tid : u64) (key : u64)
+| EvAbort  (tid : u64).
+
+Definition head_commit (tid : u64) (mods : gmap u64 u64) (l : list event) :=
+  head l = Some (EvCommit tid mods).
+
+Definition head_read (tid : u64) (key : u64) (l : list event) :=
+  head l = Some (EvRead tid key).
+
+Definition head_abort (tid : u64) (l : list event) :=
+  head l = Some (EvAbort tid).
+
+Definition no_commit_abort (tid : u64) (l : list event) :=
+  (∀ mods, EvCommit tid mods ∉ l) ∧
+  (EvAbort tid ∉ l).
+
+Definition first_abort (tid : u64) (l : list event) :=
+  ∃ e lp ls,
+    e = EvAbort tid ∧
+    l = lp ++ e :: ls ∧
+    no_commit_abort tid lp.
+
+Definition compatible (tid : u64) (mods : gmap u64 u64) (e : event) :=
+  match e with
+  | EvCommit tid' mods' => (int.Z tid') < (int.Z tid) ∨ (dom mods) ∩ (dom mods') = ∅
+  | EvRead tid' key => (int.Z tid') ≤ (int.Z tid) ∨ key ∉ (dom mods)
+  | EvAbort tid' => True
+  end.
+
+Instance compatible_dec tid mods e : Decision (compatible tid mods e).
+Proof. destruct e; simpl; apply _. Defined.
+
+Definition incompatible (tid : u64) (mods : gmap u64 u64) (e : event) := not (compatible tid mods e).
+
+Instance incompatible_dec tid mods e : Decision (incompatible tid mods e).
+Proof. destruct e; simpl; apply _. Defined.
+
+Definition compatible_all (tid : u64) (mods : gmap u64 u64) (l : list event) :=
+  Forall (compatible tid mods) l.
+
+Definition incompatible_exists (tid : u64) (mods : gmap u64 u64) (l : list event) :=
+  Exists (incompatible tid mods) l.
+
+Definition first_commit (tid : u64) (mods : gmap u64 u64) (l lp ls : list event) (e : event) :=
+  e = EvCommit tid mods ∧
+  l = lp ++ e :: ls ∧
+  no_commit_abort tid lp.
+
+Definition first_commit_incompatible (tid : u64) (mods : gmap u64 u64) (l : list event) :=
+  ∃ e lp ls,
+    first_commit tid mods l lp ls e ∧
+    incompatible_exists tid mods lp.
+
+Definition first_commit_compatible (tid : u64) (mods : gmap u64 u64) (l : list event) :=
+  ∃ e lp ls,
+    first_commit tid mods l lp ls e ∧
+    compatible_all tid mods lp.
+
+Definition is_commit_abort_tid (tid : u64) (e : event) : Prop :=
+  match e with
+  | EvCommit tid' _ => tid = tid'
+  | EvAbort tid' => tid = tid'
+  | _ => False
+  end.
+
+Instance is_commit_abort_dec tid e : Decision (is_commit_abort_tid tid e).
+Proof. destruct e; simpl; apply _. Defined.
+
+Lemma is_commit_abort_tid_lor tid e :
+  is_commit_abort_tid tid e ->
+  (∃ mods, e = EvCommit tid mods) ∨ e = EvAbort tid.
+Proof. intros. destruct e; set_solver. Qed.
+
+Fixpoint find_max_prefix (tid : u64) (lp ls : list event) : (list event * list event) :=
+  match ls with
+  | [] => (lp, ls)
+  | hd :: tl => if decide (is_commit_abort_tid tid hd)
+              then (lp, ls)
+              else find_max_prefix tid (lp ++ [hd]) tl
+  end.
+
+Lemma spec_find_max_prefix tid lp ls :
+  ∃ ls1 ls2,
+    (lp ++ ls1, ls2) = find_max_prefix tid lp ls ∧
+    ls = ls1 ++ ls2 ∧
+    no_commit_abort tid ls1 ∧
+    (match head ls2 with
+     | Some e => is_commit_abort_tid tid e
+     | _ => True
+     end).
+Proof.
+  generalize dependent lp.
+  unfold no_commit_abort.
+  induction ls as [| e ls IHls]; intros lp; simpl.
+  - exists [], [].
+    split; first by rewrite app_nil_r.
+    set_solver.
+  - case_decide.
+    + exists [], (e :: ls).
+      split; first by rewrite app_nil_r.
+      set_solver.
+    + destruct (IHls (lp ++ [e])) as (ls1 & ls2 & Heq & Hls2 & Hnca & Hhead).
+      exists ([e] ++ ls1), ls2.
+      rewrite -Heq.
+      split; first by rewrite app_assoc.
+      split; set_solver.
+Qed.
+
+Inductive tcform :=
+| NCA
+| FA
+| FCI (mods : gmap u64 u64)
+| FCC (mods : gmap u64 u64).
+
+Definition peek (tid : u64) (l : list event) : tcform :=
+  let (lp, ls) := find_max_prefix tid [] l
+  in match head ls with
+     | None => NCA
+     | Some e => match e with
+                | EvCommit _ mods => if decide (compatible_all tid mods lp) then FCC mods else FCI mods
+                | _ => FA
+                end
+     end.
+
+Theorem spec_peek tid l :
+  match peek tid l with
+  | NCA => no_commit_abort tid l
+  | FA => first_abort tid l
+  | FCI mods => first_commit_incompatible tid mods l
+  | FCC mods => first_commit_compatible tid mods l
+  end.
+Proof.
+  unfold peek.
+  destruct (spec_find_max_prefix tid [] l) as (lp & ls & Hspec & Hl & Hnca & Hls).
+  rewrite -Hspec.
+  destruct (head ls) eqn:Els.
+  - destruct e eqn:Ee.
+    + simpl.
+      apply is_commit_abort_tid_lor in Hls.
+      destruct Hls as [[mods' Hls] | Hls]; last set_solver.
+      inversion Hls. subst tid0 mods'.
+      assert (Hfc : first_commit tid mods l lp (tail ls) e).
+      { unfold first_commit.
+        split; first done.
+        split; last done.
+        rewrite Hl.
+        f_equal.
+        rewrite Ee.
+        by apply hd_error_tl_repr.
+      }
+      case_decide.
+      * unfold first_commit_compatible.
+        exists (EvCommit tid mods), lp, (tail ls).
+        by rewrite Ee in Hfc.
+      * unfold first_commit_incompatible.
+        exists (EvCommit tid mods), lp, (tail ls).
+        unfold compatible_all in H.
+        apply not_Forall_Exists in H; last apply _.
+        by rewrite Ee in Hfc.
+    + unfold is_commit_abort_tid in Hls. set_solver.
+    + apply is_commit_abort_tid_lor in Hls.
+      destruct Hls; first set_solver.
+      inversion H. subst tid0.
+      unfold first_abort.
+      exists (EvAbort tid), lp, (tail ls).
+      split; first done.
+      split; last done.
+      rewrite Hl.
+      f_equal.
+      by apply hd_error_tl_repr.
+  - apply head_None in Els.
+    rewrite Els in Hl. rewrite app_nil_r in Hl. by rewrite Hl.
+Qed.
+
+Lemma no_commit_abort_false (tid : u64) (l : list event) :
+  no_commit_abort tid l ->
+  (∃ mods, head_commit tid mods l) ∨ (head_abort tid l) ->
+  False.
+Proof.
+  intros [HnotinC HnotinA] [[mods Hhead] | Hhead]; apply head_Some_elem_of in Hhead; set_solver.
+Qed.
+
+Lemma head_middle {X} (l lp ls : list X) (x : X) :
+  l = lp ++ x :: ls ->
+  head l = head (lp ++ [x]).
+Proof.
+  intros Hl. rewrite Hl. destruct lp; auto.
+Qed.
+
+Lemma first_abort_false (tid : u64) (mods : gmap u64 u64) (l : list event) :
+  first_abort tid l ->
+  head_commit tid mods l ->
+  False.
+Proof.
+  intros (e & lp & ls & He & Hl & HnotinC & _) Hhead.
+  unfold head_commit in Hhead.
+  rewrite (head_middle _ _ _ _ Hl) in Hhead.
+  apply head_Some_elem_of in Hhead.
+  set_solver.
+Qed.
+
+Lemma first_commit_false (tid : u64) (mods : gmap u64 u64) (l lp ls : list event) (e : event) :
+  first_commit tid mods l lp ls e ->
+  head_abort tid l ->
+  False.
+Proof.
+  intros (He & Hl & _ & HnotinA) Hhead.
+  unfold head_abort in Hhead.
+  rewrite (head_middle _ _ _ _ Hl) in Hhead.
+  apply head_Some_elem_of in Hhead.
+  set_solver.
+Qed.
+
+Lemma safe_extension (tid tid' : u64) (mods : gmap u64 u64) (key : u64) (l : list event) :
+  first_commit_compatible tid mods l ->
+  head_read tid' key l ->
+  key ∈ (dom mods) ->
+  (int.Z tid') ≤ (int.Z tid).
+Proof.
+  intros (e & lp & ls & (He & Hl & _) & Hcomp) Hhead Hin.
+  unfold head_read in Hhead.
+  rewrite (head_middle _ _ _ _ Hl) in Hhead.
+  destruct lp; first set_solver.
+  simpl in Hhead.
+  inversion Hhead.
+  unfold compatible_all in Hcomp.
+  rewrite Forall_forall in Hcomp.
+  destruct (Hcomp (EvRead tid' key)); [| done | done].
+  rewrite H0.
+  apply elem_of_list_here.
+Qed.
+
+Lemma first_commit_incompatible_false (tid : u64) (mods : gmap u64 u64) (l : list event) :
+  first_commit_incompatible tid mods l ->
+  head_commit tid mods l ->
+  False.
+Proof.
+  intros (e & lp & ls & (_ & Hl & [HnotinC _]) & Hincomp) Hhead.
+  destruct lp; first by apply Exists_nil in Hincomp.
+  unfold head_commit in Hhead.
+  set_solver.
+Qed.
+
+End event.
+
 
 Section mvccinv.
 Context `{!heapGS Σ, !mvcc_ghostG Σ}.
